updates

theories/Examples/ConcurrentHashTable.v
@@ -12,6 +12,8 @@
 From Stdlib Require Import List Bool Nat.
 From Crane Require Extraction.
 From Crane Require Import Monads.ITree Monads.IODefs Monads.STMDefs.
+From Crane Require Import Utils.WithPost.
+From ITree Require Import Eq Props.HasPost.
 
 Import ListNotations.
 Set Implicit Arguments.
@@ -20,9 +22,6 @@ Set Implicit Arguments.
 Axiom nat_of_int : int -> nat.
 Crane Extract Inlined Constant nat_of_int => "static_cast<unsigned int>(%a0)".
 *)
-
-From ITree Require Import Eq Props.HasPost.
-From Paco Require Import paco.
 
 Module CHT.
 
@@ -146,17 +145,6 @@ Definition mk_buckets (num : nat) : itree runStmIOE (list (TVar (list (K * V))))
         f (b :: buckets) n'
     end) [] num.
 
-Lemma has_post_subrel : forall {E R} (t : itree E R) (P Q : R -> Prop),
-  (forall x, P x -> Q x) ->
-  has_post t P ->
-  has_post t Q.
-Proof.
-  intros.
-  eapply eutt_subrel, H0.
-  intros ??.
-  apply H.
-Qed.
-
 Lemma mk_buckets_length : forall n, has_post (mk_buckets n) (fun buckets => length buckets = n).
 Proof.
   intros.
@@ -172,72 +160,6 @@ Proof.
     cbn. rewrite plus_n_Sm.
     apply IHn.
 Qed.
-
-
-
-Lemma has_post_eta {E R} {P : R -> Prop} (t : itree E R) : has_post t P -> has_post (go (observe t)) P.
-Proof.
-  intros.
-  rewrite <- itree_eta.
-  assumption.
-Qed.
-
-Lemma has_post_inv_Ret {E R} {P : R -> Prop} (r : R) : has_post ((Ret r) : itree E R) P -> P r.
-Proof.
-  intros.
-  apply eqit_inv_Ret in H.
-  apply H.
-Qed.
-
-Lemma has_post_inv_Tau {E R} {P : R -> Prop} (t : itree E R) : has_post (Tau t) P -> has_post t P.
-Proof.
-  intros.
-  apply eqit_inv_Tau in H.
-  apply H.
-Qed.
-
-Lemma has_post_inv_Vis {E R} {P : R -> Prop} {X} (e : E X) (k : X -> itree E R) : has_post (Vis e k) P -> forall x, has_post (k x) P.
-Proof.
-  intros.
-  eapply eqit_inv_Vis in H.
-  apply H.
-Qed.
-
-CoFixpoint with_post {E R} {P : R -> Prop} (t : itree E R) (pf : has_post t P) : itree E {x:R | P x} :=
-  let ot := observe t in
-  let pf' := has_post_eta pf in
-  (match ot return ot = observe t -> _ with
-  | RetF r => fun Heqot => Ret (exist P r (has_post_inv_Ret (eq_ind_r (fun ot => has_post (go ot) P) pf' Heqot)))
-  | TauF t => fun Heqot => Tau (@with_post E R P t (has_post_inv_Tau (eq_ind_r (fun ot => has_post (go ot) P) pf' Heqot)))
-  | VisF e k => fun Heqot => Vis e (fun x => @with_post E R P (k x) (has_post_inv_Vis (eq_ind_r (fun ot => has_post (go ot) P) pf' Heqot) x))
-  end) eq_refl.
-
-Arguments with_post : clear implicits.
-Arguments with_post {E R P} (t pf).
-
-Notation with_post_ P t pf :=
-  (let ot := observe t in
-   let pf' := has_post_eta pf in
-   (match ot return ot = observe t -> _ with
-    | RetF r => fun Heqot => Ret (exist P r (has_post_inv_Ret (eq_ind_r (fun ot => has_post (go ot) P) pf' Heqot)))
-    | TauF t => fun Heqot => Tau (@with_post _ _ P t (has_post_inv_Tau (eq_ind_r (fun ot => has_post (go ot) P) pf' Heqot)))
-    | VisF e k => fun Heqot => Vis e (fun x => @with_post _ _ P (k x) (has_post_inv_Vis (eq_ind_r (fun ot => has_post (go ot) P) pf' Heqot) x))
-    end) eq_refl).
-
-
-
-Lemma unfold_with_post {E R} (P : R -> Prop) (t : itree E R) (pf : has_post t P) :
-  with_post t pf ≅ with_post_ P t pf.
-Proof.
-  apply observing_sub_eqit; constructor; reflexivity.
-Qed.
-
-
-Lemma with_post_proj1 {E R} {P : R -> Prop} (t : itree E R) (pf : has_post t P) :
-  ITree.map (@proj1_sig R P) (with_post t pf) ≅ t.
-Proof.
-Abort.
-
 
 (* Create a new table with at least one bucket; stores eqb/hash in the record *)
 Definition new_hash
