theories/Monads/STM/AtomicTransactionsAxiom.v
@@ -1,0 +1,57 @@
+From Crane.Monads Require Import ITree STMDefsAxiom STM.Atomic STM.TransactionDefs STM.ForkDefs STM.WriteLog.
+From Crane.Utils Require Import HMap HAList.
+
+From Stdlib Require Import List Classes.EquivDec.
+
+Import ListNotations.
+
+From ITree Require Import Basics.Basics Basics.CategoryOps Events.FailFacts.
+
+Import Basics.Monads.
+
+Axiom tid : Type.
+Axiom tid_eq_dec : forall (i1 i2 : tid), i1 = i2 \/ i1 <> i2.
+
+Variant transactionImplE E : Type -> Type :=
+| NewTransactionID : transactionImplE E tid
+| TransactionEvent : forall X, E X -> tid -> transactionImplE E X
+| AbortTransaction : tid -> transactionImplE E unit
+| CommitTransaction : tid -> transactionImplE E unit.
+
+Definition embed_transaction_events (t : tid) : stmE ~> failT (itree (transactionImplE tvarE)) :=
+  fun _ e =>
+    match e with
+    | inl1 Retry => Ret None
+    | inr1 e => v <- trigger (TransactionEvent _ _ e t);; Ret (Some v)
+    end.
+
+(* Implements transactions by executing them atomically (blocks all other threads from executing until it is finished) *)
+Definition h_atomic_transactions : transactionE stmE ~> atomicE (transactionImplE tvarE) :=
+  fun _ e =>
+    match e with
+    | Transaction t =>
+        Atomic (i <- trigger (NewTransactionID _) ;;
+                res <- interp (embed_transaction_events i) t ;;
+                match res with
+                | Some a =>
+                    trigger (CommitTransaction _ i) ;;
+                    Ret (Some a)
+                | None =>
+                    trigger (AbortTransaction _ i) ;;
+                    Ret None
+                end)
+    end.
+
+Definition atomic_transactions {E} `{atomicE (transactionImplE tvarE) -< E} : transactionE stmE ~> itree E :=
+  fun _ e => trigger (h_atomic_transactions _ e).
+
+Definition run_atomic_transactions
+  (t1 : itree (transactionE stmE +' forkE) unit):
+  itree void1 (halist (pkey K nat) (pkey_type V) * unit) :=
+  let t2 := interp (case_ (C := IFun) (bif := sum1) (c := itree (forkE +' atomicE (tvarE V) +' tvarE V))
+                          atomic_transactions
+                          (fun _ e => trigger e))
+                   t1 in
+  let t3 : itree (tvarE V) unit := run_atomic (schedule_rr [t2]) in
+  let t4 : stateT _ _ _ := interp (handle_tvars _ _) t3 in
+  t4 HMap.empty.
