theories/Monads/STM/WriteLogAxiom.v
@@ -1,0 +1,69 @@
+From Crane Require Import Monads.ITree Monads.STMDefsAxiom Utils.HMap.
+
+From ExtLib Require Import Structures.Reducible.
+
+From ITree Require Import Basics.Basics Events.FailFacts.
+
+Import Basics.Monads.
+
+From Stdlib Require Import List.
+Import ListNotations.
+
+Definition commit_log {M} `{Foldable M (sigT (fun X => TVar X * X)%type)} {E} `{H : tvarE -< E} : M -> itree E unit :=
+  fold (fun '(existT _ X (x, v)) acc => Vis (subevent (H := H) _ (WriteTVar x v)) (fun _ => acc)) (Ret tt).
+
+Variant tvar_log_entry : Type :=
+| tvar_log_new {A} (x : TVar A) (a : A)
+| tvar_log_write {A} (x : TVar A) (a : A).
+
+Definition tvar_log : Type := list tvar_log_entry.
+
+Fixpoint log_write (l : tvar_log) {A} (x : TVar A) (v : A) : tvar_log :=
+  match l with
+  | [] => _
+  | tvar_log_new y a :: l' => _
+  | tvar_log_write y a :: l' => _
+  end.
+
+Definition handle_tvar_log {M} {E} `{H : tvarE -< E}
+  (m : M) : forall {A}, tvarE A -> itree E (A * M) :=
+  fun _ t =>
+    match t with
+    | NewTVar k v => Vis (subevent (H := H) _ (NewTVar k v)) (fun tv => Ret (tv, m))
+    | ReadTVar tv =>
+        (let '(mk_tvar _ n k) in TVar _ T := tv return TVar V T -> itree E (T * M) in
+          match lookup (k, n) m with
+          | Some v => fun _ => Ret (v, m)
+          | None => fun tv => Vis (subevent (H := H) _ (ReadTVar tv)) (fun v => Ret (v, m))
+          end) tv
+    | WriteTVar (mk_tvar _ n k) v => Ret (tt, add (k, n) v m)
+    end.
+
+Definition h_stm_write_log {K} {V : K -> Type} {M} `{HMap (pkey K nat) (pkey_type V) M} {E} `{tvarE V -< E}:
+  stmE V ~> stateT M (failT (itree E)) :=
+  fun _ e m =>
+    match e with
+    | inl1 Retry => Ret None
+    | inr1 e =>
+        '(a, m) <- handle_tvar_log m e ;;
+        Ret (Some (m, a))
+    end.
+
+Definition handle_tvars {E} {K} (V : K -> Type) M
+  `{HMap (pkey K nat) (pkey_type V) M} `{Foldable M (sigT (@pkey_type K nat V))}:
+  tvarE V ~> stateT M (itree E) :=
+  fun _ t m =>
+    match t with
+    | NewTVar k v =>
+        let n := S (fold (fun '(existT _ (_, n) _) acc => max n acc) 0 m) in
+        Ret (add (k, n) v m, mk_tvar V n k)
+    | ReadTVar x =>
+        let '(mk_tvar _ n k) := x in
+        match lookup (k, n) m with
+        | Some v => Ret (m, v)
+        | None => ITree.spin (* error *)
+        end
+    | WriteTVar x v =>
+        (let '(mk_tvar _ n k) := x in
+         fun (v : V k) => Ret (add (k, n) v m, tt)) v
+    end.
