theories/Utils/WithPost.v
@@ -1,0 +1,77 @@
+From ITree Require Import ITree Eq Props.HasPost.
+
+#[local] Open Scope itree_scope.
+
+Lemma has_post_eta {E R} {P : R -> Prop} (t : itree E R) : has_post t P -> has_post (go (observe t)) P.
+Proof.
+  intros.
+  rewrite <- itree_eta.
+  assumption.
+Qed.
+
+Lemma has_post_inv_Ret {E R} {P : R -> Prop} (r : R) : has_post ((Ret r) : itree E R) P -> P r.
+Proof.
+  intros.
+  apply eqit_inv_Ret in H.
+  apply H.
+Qed.
+
+Lemma has_post_inv_Tau {E R} {P : R -> Prop} (t : itree E R) : has_post (Tau t) P -> has_post t P.
+Proof.
+  intros.
+  apply eqit_inv_Tau in H.
+  apply H.
+Qed.
+
+Lemma has_post_inv_Vis {E R} {P : R -> Prop} {X} (e : E X) (k : X -> itree E R) : has_post (Vis e k) P -> forall x, has_post (k x) P.
+Proof.
+  intros.
+  eapply eqit_inv_Vis in H.
+  apply H.
+Qed.
+
+CoFixpoint with_post {E R} {P : R -> Prop} (t : itree E R) (pf : has_post t P) : itree E {x:R | P x} :=
+  let ot := observe t in
+  let pf' := has_post_eta _ pf in
+  (match ot return ot = observe t -> _ with
+  | RetF r => fun Heqot => Ret (exist P r (has_post_inv_Ret _ (eq_ind_r (fun ot => has_post (go ot) P) pf' Heqot)))
+  | TauF t => fun Heqot => Tau (@with_post E R P t (has_post_inv_Tau _ (eq_ind_r (fun ot => has_post (go ot) P) pf' Heqot)))
+  | VisF e k => fun Heqot => Vis e (fun x => @with_post E R P (k x) (has_post_inv_Vis _ _ (eq_ind_r (fun ot => has_post (go ot) P) pf' Heqot) x))
+  end) eq_refl.
+
+Arguments with_post : clear implicits.
+Arguments with_post {E R P} (t pf).
+
+Notation with_post_ P t pf :=
+  (let ot := observe t in
+   let pf' := has_post_eta _ pf in
+   (match ot return ot = observe t -> _ with
+    | RetF r => fun Heqot => Ret (exist P r (has_post_inv_Ret _ (eq_ind_r (fun ot => has_post (go ot) P) pf' Heqot)))
+    | TauF t => fun Heqot => Tau (@with_post _ _ P t (has_post_inv_Tau _ (eq_ind_r (fun ot => has_post (go ot) P) pf' Heqot)))
+    | VisF e k => fun Heqot => Vis e (fun x => @with_post _ _ P (k x) (has_post_inv_Vis _ _ (eq_ind_r (fun ot => has_post (go ot) P) pf' Heqot) x))
+    end) eq_refl).
+
+
+
+Lemma unfold_with_post {E R} (P : R -> Prop) (t : itree E R) (pf : has_post t P) :
+  with_post t pf ≅ with_post_ P t pf.
+Proof.
+  apply observing_sub_eqit; constructor; reflexivity.
+Qed.
+
+
+Lemma with_post_proj1 {E R} {P : R -> Prop} (t : itree E R) (pf : has_post t P) :
+  ITree.map (@proj1_sig R P) (with_post t pf) ≅ t.
+Proof.
+Abort.
+
+Lemma has_post_subrel : forall {E R} (t : itree E R) (P Q : R -> Prop),
+  (forall x, P x -> Q x) ->
+  has_post t P ->
+  has_post t Q.
+Proof.
+  intros.
+  eapply eutt_subrel, H0.
+  intros ??.
+  apply H.
+Qed.
